Source/DafnyStandardLibraries/examples2/Iterators.dfy
@@ -1,0 +1,116 @@
+module ActionsExamples {
+  import opened Std.Actions
+  import opened Std.Producers
+  import opened Std.Consumers
+  import opened Std.Wrappers
+
+  // Adapting an iterator to a producer
+
+  iterator FibonacciIterator() yields (current: nat)
+    ensures false
+  {
+    current := 0;
+    yield;
+
+    var prev: nat := 0;
+    current := 1;
+    while true {
+      var next := prev + current;
+      prev := current;
+      current := next;
+      yield;
+    }
+  }
+
+  @AssumeCrossModuleTermination
+  class FibonacciProducer extends IProducer<nat> {
+
+    const iter: FibonacciIterator
+
+    ghost predicate Valid()
+      reads this, Repr
+      ensures Valid() ==> this in Repr
+      ensures Valid() ==> ValidHistory(history)
+      decreases height, 0
+    {
+      && this in Repr
+      && iter in Repr
+      && this !in iter._reads && iter._reads <= Repr
+      && this !in iter._modifies && iter._modifies <= Repr
+      && this !in iter._new && iter._new <= Repr
+      && iter.Valid()
+    }
+
+    constructor () 
+      ensures Valid()
+      ensures fresh(Repr)
+    {
+      this.iter := new FibonacciIterator();
+      new;
+      Repr := {this, iter} + NonNullElements(iter._reads) + NonNullElements(iter._modifies) + NonNullElements(iter._new);
+      height := 0;
+    }
+
+    function NonNullElements(s: set<object?>): set<object> {
+      s - {null}
+    }
+
+    ghost predicate ValidHistory(history: seq<((), nat)>)
+      decreases height
+    {
+      true
+    }
+    ghost predicate ValidInput(history: seq<((), nat)>, next: ())
+      decreases height
+    {
+      true
+    }
+    twostate predicate ValidOutput(history: seq<((), nat)>, nextInput: (), new nextOutput: nat)
+      decreases height
+      ensures ValidOutput(history, nextInput, nextOutput) ==> ValidHistory(history + [(nextInput, nextOutput)])
+    {
+      ValidHistory(history + [(nextInput, nextOutput)])
+    }
+
+    method Invoke(i: ()) returns (o: nat)
+      requires Requires(i)
+      modifies Modifies(i)
+      decreases Decreases(i).Ordinal()
+      ensures Ensures(i, o)
+    {
+      assert Valid();
+      var more := iter.MoveNext();
+      assert history == old(history);
+      assert more;
+
+      o := iter.current;
+
+      UpdateHistory(i, o);
+      Repr := {this, iter} + NonNullElements(iter._reads) + NonNullElements(iter._modifies) + NonNullElements(iter._new);
+    }
+
+  }
+
+  method PrintOutFibonnaci() {
+    var iproducer := new FibonacciProducer();
+    var iproducerTotalProof := new DefaultTotalActionProof(iproducer);
+    var producer := new LimitedProducer(iproducer, 10, iproducerTotalProof);
+
+    while true 
+      invariant producer.Valid()
+      invariant fresh(producer.Repr)
+      decreases producer.Remaining()
+    {
+      var next := producer.Next();
+      if next.None? {
+        break;
+      }
+
+      print next.value, "\n";
+    }
+  }
+
+  method Main() {
+    PrintOutFibonnaci();
+  }
+}
